new_proof/RefinementDenotationProp.v
@@ -185,6 +185,24 @@ Qed.
 
 (*       rewrite IHΓ in H6. *)
 
+Inductive wf_ctx: listctx rty -> Prop :=
+| wf_ctx_nil: wf_ctx []
+| wf_ctx_cons_ubase: forall Γ x b n d ϕ,
+    wf_ctx Γ ->
+    ~ (⟦ [v: b | n | d | ϕ ] ⟧{ Γ } terr) ->
+    ok_dctx ∅ (Γ ++ [(x, [v: b | n | d | ϕ])]) ->
+    wf_ctx (Γ ++ [(x, [v: b | n | d | ϕ ])])
+| wf_ctx_cons: forall Γ x τ,
+    wf_ctx Γ ->
+    not_underbasety τ ->
+    ok_dctx ∅ (Γ ++ [(x, τ)]) ->
+    wf_ctx (Γ ++ [(x, τ)]).
+
+Definition wf (Γ: listctx rty) (τ: rty) :=
+  wf_ctx Γ /\ closed_rty 0 (ctxdom Γ) τ.
+
+Notation " Γ '⊢WF' τ " := (wf Γ τ) (at level 20, τ constr, Γ constr).
+
 Fixpoint random_inhabitant (τ: rty) :=
   match τ with
   | {v: _ | _ | _ | _ } => terr
@@ -194,393 +212,264 @@ Fixpoint random_inhabitant (τ: rty) :=
   | τ1 ⤑ τ2 => vlam (rty_erase τ1) (random_inhabitant τ2)
   end.
 
-Ltac lc_solver2 :=
-  match goal with
-    | [H: lc (tlete ?u _) |- lc ?u] => invclear H; auto
-    end || lc_solver1.
-
-Lemma subst_subst_tm: ∀ (x : atom) (u_x : value) (y : atom) (u_y: value) (e: tm),
-    x ≠ y → y ∉ fv_value u_x →
-    {x := u_x }t ({y := u_y }t e) = {y := {x := u_x }v u_y }t ({x := u_x }t e).
-Proof.
-  intros x u_x y u_y e Hxy Hyux. apply (tm_mutual_rec
-           (fun (e: value) => {x := u_x }v ({y := u_y }v e) = {y := {x := u_x }v u_y }v ({x := u_x }v e))
-           (fun (e: tm) => {x := u_x }t ({y := u_y }t e) = {y := {x := u_x }v u_y }t ({x := u_x }t e))
-        ); simpl; intros; auto;
-  try (rewrite H; auto; rewrite H0; auto; rewrite H1; auto);
-  try (repeat var_dec_solver; rewrite subst_fresh_value; auto).
-Qed.
-
-Lemma subst_subst_value: ∀ (x : atom) (u_x : value) (y : atom) (u_y e : value),
-    x ≠ y → y ∉ fv_value u_x →
-    {x := u_x }v ({y := u_y }v e) = {y := {x := u_x }v u_y }v ({x := u_x }v e).
-Proof.
-  intros x u_x y u_y e Hxy Hyux. apply (value_mutual_rec
-           (fun (e: value) => {x := u_x }v ({y := u_y }v e) = {y := {x := u_x }v u_y }v ({x := u_x }v e))
-           (fun (e: tm) => {x := u_x }t ({y := u_y }t e) = {y := {x := u_x }v u_y }t ({x := u_x }t e))
-        ); simpl; intros; auto;
-  try (rewrite H; auto; rewrite H0; auto; rewrite H1; auto);
-  try (repeat var_dec_solver; rewrite subst_fresh_value; auto).
-Qed.
-
-Lemma fv_of_subst_value: forall x (u e: value), fv_value ({x := u }v e) ⊆ (fv_value e ∖ {[x]}) ∪ fv_value u.
-Proof.
-  intros x u. apply (value_mutual_rec
-           (fun (e: value) => fv_value ({x := u }v e) ⊆ fv_value e ∖ {[x]} ∪ fv_value u)
-           (fun (e: tm) => fv_tm ({x := u }t e) ⊆ fv_tm e ∖ {[x]} ∪ fv_value u)
-        ); simpl; intros; auto; repeat var_dec_solver; set_solver.
-Qed.
-
-Lemma fv_of_subst_tm: forall x (u : value) (e: tm), fv_tm ({x := u }t e) ⊆ (fv_tm e ∖ {[x]}) ∪ fv_value u.
-Proof.
-  intros x u. apply (tm_mutual_rec
-           (fun (e: value) => fv_value ({x := u }v e) ⊆ fv_value e ∖ {[x]} ∪ fv_value u)
-           (fun (e: tm) => fv_tm ({x := u }t e) ⊆ fv_tm e ∖ {[x]} ∪ fv_value u)
-        ); simpl; intros; auto; repeat var_dec_solver; set_solver.
-Qed.
-
-Lemma fv_of_subst_value_closed: forall x (u e: value),
-    fv_value u ≡ ∅ ->
-    fv_value ({x := u }v e) = (fv_value e ∖ {[x]}).
-Proof.
-  intros x u.
-  apply (value_mutual_rec
-           (fun (e: value) =>
-              fv_value u ≡ ∅ -> fv_value ({x := u }v e) = fv_value e ∖ {[x]})
-           (fun (e: tm) =>
-              fv_value u ≡ ∅ -> fv_tm ({x := u }t e) = fv_tm e ∖ {[x]})
-        ); simpl; intros; auto; repeat var_dec_solver; set_solver.
-Qed.
-
-Lemma fv_of_subst_tm_closed: forall x (u: value) e,
-    fv_value u ≡ ∅ -> fv_tm ({x := u }t e) = (fv_tm e ∖ {[x]}).
-Proof.
-  intros x u.
-  apply (tm_mutual_rec
-           (fun (e: value) =>
-              fv_value u ≡ ∅ -> fv_value ({x := u }v e) = fv_value e ∖ {[x]})
-           (fun (e: tm) =>
-              fv_value u ≡ ∅ -> fv_tm ({x := u }t e) = fv_tm e ∖ {[x]})
-        ); simpl; intros; auto; repeat var_dec_solver; set_solver.
-Qed.
-
-Lemma tm_msubst_then_subst: forall Γ env,
-    instantiation Γ env ->
-    forall (z: atom) (u: value) e, z ∉ ctxdom env -> z # u ->
-    tm_msubst env ({z := u }t e) = ({z := value_msubst env u }t (tm_msubst env e)).
-Proof.
-  intros Γ env Hi. unfold closed_value.
-  induction Hi; simpl; intros; mydestr; auto.
-  - setoid_rewrite subst_subst_tm; try basic_typing_solver.
-    rewrite IHHi; try fast_set_solver. simpl.
-    apply basic_typing_contains_fv_value in H.
-    pose (fv_of_subst_value x v u). set_solver.
-Qed.
-
-Lemma value_msubst_then_subst: forall Γ env,
-    instantiation Γ env ->
-    forall (z: atom) (u: value) e, z ∉ ctxdom env -> z # u ->
-    value_msubst env ({z := u }v e) = ({z := value_msubst env u }v (value_msubst env e)).
-Proof.
-  intros Γ env Hi. unfold closed_value.
-  induction Hi; simpl; intros; mydestr; auto.
-  - setoid_rewrite subst_subst_value; try basic_typing_solver.
-    rewrite IHHi; try fast_set_solver.
-    apply basic_typing_contains_fv_value in H.
-    pose (fv_of_subst_value x v u). set_solver.
-Qed.
-
-Lemma tm_msubst_then_open: forall Γ env,
-    instantiation Γ env ->
-    forall (u: value) e, ctxdom env ∩ fv_value u = ∅ ->
-                    (tm_msubst env e) ^t^ u = (tm_msubst env (e ^t^ u)).
-Proof.
-  intros Γ env Hi.
-  induction Hi; simpl; intros; mydestr; auto.
-  - setoid_rewrite subst_open_tm; try basic_typing_solver.
-    rewrite (subst_fresh_value u).
-    rewrite IHHi; auto; set_solver.
-    set_solver.
-Qed.
-
-Lemma value_msubst_then_open: forall Γ env,
-    instantiation Γ env ->
-    forall (u: value) e, ctxdom env ∩ fv_value u = ∅ ->
-                    (value_msubst env e) ^v^ u = (value_msubst env (e ^v^ u)).
-Proof.
-  intros Γ env Hi.
-  induction Hi; simpl; intros; mydestr; auto.
-  - setoid_rewrite subst_open_value; try basic_typing_solver.
-    rewrite (subst_fresh_value u).
-    rewrite IHHi; auto; set_solver.
-    set_solver.
-Qed.
-
-Lemma tm_msubst_then_open_closed: forall Γ env,
-    instantiation Γ env ->
-    forall (u: value) e, fv_value u ≡ ∅ ->
-                    (tm_msubst env e) ^t^ u = (tm_msubst env (e ^t^ u)).
-Proof.
-  intros. eapply tm_msubst_then_open; eauto. set_solver.
-Qed.
-
-Lemma value_msubst_then_open_closed: forall Γ env,
-    instantiation Γ env ->
-    forall (u: value) e, fv_value u ≡ ∅ ->
-                    (value_msubst env e) ^v^ u = (value_msubst env (e ^v^ u)).
-Proof.
-   intros. eapply value_msubst_then_open; eauto. set_solver.
-Qed.
-
-Ltac basic_typing_solver5 :=
-  repeat (simpl; (basic_typing_solver4 ||
-                    match goal with
-                    | [H: _ ⊢t (tvalue _) ⋮t _  |- _ ] => invclear H; eauto
-                    | [H: ?Γ ⊢t ?e ⋮t _, H': ?z ∉ ctxdom ?Γ  |- ?z ∉ fv_tm ?e ] =>
-                        apply basic_typing_contains_fv_tm in H; simpl in H; fast_set_solver
-                    | [H: ?Γ ⊢t ?e ⋮v _, H': ?z ∉ ctxdom ?Γ  |- ?z ∉ fv_value ?e ] =>
-                        apply basic_typing_contains_fv_value in H; fast_set_solver
-                    | [H: ?Γ ⊢t tlete ?u _ ⋮t _ |- ?Γ ⊢t ?u ⋮t _ ] => invclear H; eauto
-                    | [H: ?Γ ⊢t tlete (tvalue ?u) _ ⋮t _ |- ?Γ ⊢t ?u ⋮v _ ] => invclear H; eauto
-                    end)).
-
-Lemma instantiation_implies_tm_msubst_closed:
-  forall Γ env, instantiation Γ env -> ∀ e T, Γ ⊢t e ⋮t T -> closed_tm (tm_msubst env e).
-Proof.
-  intros Γ env Hi. induction Hi; simpl; intros; basic_typing_solver5.
-  assert (c ⊢t ({x := v }t e0) ⋮t T0) by basic_typing_solver5; eauto.
-Qed.
-
-Lemma instantiation_implies_value_msubst_closed:
-  forall Γ env, instantiation Γ env -> ∀ (e: value) T, Γ ⊢t e ⋮v T -> closed_value (value_msubst env e).
-Proof.
-  intros Γ env Hi. induction Hi; simpl; intros; basic_typing_solver5.
-  assert (c ⊢t ({x := v }v e0) ⋮v T0) by basic_typing_solver5; eauto.
-Qed.
-
-Global Hint Unfold closed_value: core.
-Global Hint Unfold closed_tm: core.
-
-Ltac isolver :=
-  instantiation_regular_solver || (basic_typing_solver5; lc_solver2).
-
-Lemma tlete_reduce_to_subst: forall (u: value) z e,
-    lc u -> lc e ->
-    tlete u (z \t\ e) ↪* {z := u }t e.
-Proof.
-  intros.
-  apply multistep_trans with (y := (z \t\ e) ^t^ u).
-  apply multistep_R. econstructor; isolver.
-  setoid_rewrite subst_as_close_open_tm; eauto.
-  apply subst_lc_tm; auto.
-  setoid_rewrite subst_as_close_open_tm; eauto.
-  eapply multistep_refl. apply subst_lc_tm; auto; isolver.
-Qed.
-
-Lemma termR_let_one_step_from_basic_type: forall Γ (u: value) (z: atom) e T,
-    lc e -> z ∉ ctxdom Γ ->
-    Γ ⊢t (tlete u (z \t\ e)) ⋮t T ->
-    (tlete u (z \t\ e)) <-<{ Γ; T} ({z := u }t e).
-Proof.
-  intros. constructor; auto.
-  - eapply multi_preservation; eauto.
-    apply tlete_reduce_to_subst; isolver.
-  - unfold termRraw. intros. msubst_simpl.
-    rewrite lete_step_spec in H3; simpl; mydestr.
-    rewrite value_reduce_to_value_implies_same in H4; mydestr; subst.
-    invclear H1.
-    assert (closed_value (value_msubst env u)) by
-    (eapply instantiation_implies_value_msubst_closed; eauto; basic_typing_solver5).
-    assert (z ∉ ctxdom env) by instantiation_regular_solver.
-    erewrite tm_msubst_then_subst; eauto; try basic_typing_solver5.
-    erewrite tm_msubst_then_open_closed in H5; eauto; try basic_typing_solver5.
-    rewrite subst_as_close_open_tm in H5; eauto; try basic_typing_solver5.
-    erewrite tm_msubst_then_subst in H5; eauto; try basic_typing_solver5.
-    eapply value_msubst_closed in H1. rewrite H1 in H5; auto.
-    set_solver.
-Qed.
-
-Lemma instantiation_implies_value_msubst_lc:
-      ∀ Γ Γv, instantiation Γ Γv -> forall (e: value), lc e -> lc (value_msubst Γv e).
-Proof.
-  intros Γ Γv Hi. induction Hi; simpl; intros; auto.
-  - apply IHHi. apply subst_lc_value; basic_typing_solver3.
-Qed.
-
-Lemma termR_let_one_step_from_basic_type': forall Γ (u: value) (z: atom) e T,
-    lc e -> z ∉ ctxdom Γ ->
-    Γ ⊢t (tlete u (z \t\ e)) ⋮t T ->
-    ({z := u }t e) <-<{ Γ; T} (tlete u (z \t\ e)).
-Proof.
-  intros. constructor; auto.
-  - eapply multi_preservation; eauto.
-    apply tlete_reduce_to_subst; isolver.
-  - unfold termRraw. intros. msubst_simpl.
-    rewrite lete_step_spec. split.
-    + eapply msubst_preserves_body_tm; eauto. lc_solver.
-      setoid_rewrite subst_as_close_open_tm; eauto.
-      apply subst_lc_tm; auto.
-    + invclear H1.
-      exists (value_msubst env u). split.
-      { rewrite value_reduce_to_value_implies_same; split; auto.
-        eapply instantiation_implies_value_msubst_lc; eauto. basic_typing_solver5. }
-      assert (z ∉ ctxdom env) by instantiation_regular_solver.
-      assert (closed_value (value_msubst env u)) by
-        (eapply instantiation_implies_value_msubst_closed; eauto; basic_typing_solver5).
-      erewrite tm_msubst_then_subst in H3; eauto; try basic_typing_solver5.
-      erewrite tm_msubst_then_open_closed; eauto; try basic_typing_solver5.
-      rewrite subst_as_close_open_tm; eauto; try basic_typing_solver5.
-      erewrite tm_msubst_then_subst; eauto; try basic_typing_solver5.
-      rewrite value_msubst_closed; auto.
-      set_solver.
-Qed.
-
-Lemma let_store_tyable: forall Γ u Tu z e T,
-         Γ ⊢t u ⋮t Tu -> (Γ ++ [(z, Tu)]) ⊢t e ⋮t T -> Γ ⊢t tlete u (z \t\ e) ⋮t T.
+Lemma vlam_tyable_dummy: forall Γ e Tx T,
+  Γ ⊢t e ⋮t T -> Γ ⊢t vlam Tx e ⋮v Tx ⤍ T.
 Proof.
   intros. auto_exists_L; intros.
-  rewrite subst_as_close_open_tm; eauto; try basic_typing_solver5.
-  apply basic_has_type_renaming; try basic_typing_solver5.
+  rewrite open_rec_lc_tm; basic_typing_solver.
 Qed.
 
-Lemma rRctx_backward_over: forall Γ st z b n d ϕ (e: tm) τ,
-    not_overbasety τ ->
-    {st}⟦ τ ⟧{ Γ ++ [(z, {v: b | n | d | ϕ})] } e <->
-      (closed_rty 0 (ctxdom (Γ ++ [(z, {v: b | n | d | ϕ})]) ∪ dom aset st) τ /\
-         ok_dctx (dom aset st) (Γ ++ [(z, {v: b | n | d | ϕ})]) /\
-         (⌊Γ ++ [(z, {v: b | n | d | ϕ})]⌋*) ⊢t e ⋮t ⌊τ⌋ /\
-            (forall (u: value), {st}⟦ {v: b | n | d | ϕ} ⟧{ Γ } u -> {st}⟦ { z := u }r τ ⟧{ Γ } ({ z := u }t e))).
+Lemma vlam_implies_open_tyable: forall Γ e1 v2 Tx T,
+  Γ ⊢t v2 ⋮v Tx -> Γ ⊢t vlam Tx e1 ⋮v Tx ⤍ T -> Γ ⊢t e1 ^t^ v2 ⋮t T.
 Proof.
-  induction Γ; split; simpl; intros; denotation_simp.
-  - RD_simp. split; denotation_simp. split; auto. split; auto.
-    intros. RD_simp. apply H13 in H1. RD_simp.
-    rewrite denotation_st_update_iff_subst in H0; mydestr; auto; refinement_solver3.
-    eapply termR_perserve_rR; eauto; refinement_solver3. ctx_erase_simp4.
-    apply termR_let_one_step_from_basic_type; auto.
-    basic_typing_solver. refinement_solver3. refinement_solver. denotation_simp.
-  - constructor; try refinement_solver. intros.
-    assert (({st}⟦{v:b|n|d|ϕ}⟧{ [] }) c_x) as HH by (constructor; auto).
-    apply H3 in HH. RD_simp.
-    rewrite denotation_st_update_iff_subst; refinement_solver3.
-    split; refinement_solver3. denotation_simp.
-    eapply termR_perserve_rR; eauto; denotation_simp; refinement_solver3.
-    apply termR_let_one_step_from_basic_type'; basic_typing_solver5.
-    eapply let_store_tyable; eauto.
-  - invclear H0; denotation_simp.
-    + do 3 (split; auto). intros. invclear H0. apply ctxrR_cons_over; denotation_simp; auto.
-      admit. admit.
-      intros.
-      assert (({<[a:=c_x]> st}⟦{v:b|0|d|ϕ}⟧{Γ}) (tlete c_x (a \v\ u))) by auto.
-      assert ({<[a:=c_x]> st}⟦τ⟧{ Γ ++ [(z, {v:b|0|d|ϕ})] } (tlete c_x (a \t\ e))) by auto.
-      rewrite IHΓ in H3; mydestr.
-      assert (({<[a:=c_x]> st}⟦{v:b|0|d|ϕ}⟧{Γ}) ({a := c_x}v u)).
-      eapply termR_perserve_ctxrR; eauto.
-      assert (({st}⟦{v:b|0|d|ϕ}⟧{Γ}) (tlete c_x (a \v\ u))).
-      denotation_st_update_iff_subst
+  intros. invclear H0. auto_pose_fv x. repeat specialize_with x.
+  eapply basic_typing_subst_tm_pre in H3; eauto.
+  rewrite subst_open_tm in H3; basic_typing_solver.
+  simpl in H3. var_dec_solver.
+  rewrite subst_fresh_tm in H3; basic_typing_solver.
+Qed.
 
-      apply H10 in H0.
-    + do 3 (split; auto). intros.
-  - destruct (classic (not_overbasety r)).
-    + constructor; try refinement_solver3. admit.
-    + auto_ty_exfalso. apply ctxrR_cons_over; try refinement_solver3.
-      intros. rewrite IHΓ. split. admit. split. admit. split. admit.
-      intros. admit.
+Ltac basic_typing_solver6 :=
+  repeat (basic_typing_solver ||
+     (match goal with
+            | [H: ?Γ ⊢t vlam ?Tx ?e1 ⋮v ?Tx ⤍ ?T |- ?Γ ⊢t ?e1 ^t^ ?v2 ⋮t ?T] =>
+                apply vlam_implies_open_tyable with (Tx := Tx); eauto
+             | [ |- _ ⊢t tvalue _ ⋮t _ ⤍ _ ] => constructor; auto
+             | [ |- _ ⊢t vlam _ _ ⋮v _ ⤍ _ ] => apply vlam_tyable_dummy; eauto
+             end)).
+
+Lemma random_inhabitant_tyable: ∀ (τ: rty) Γ,
+    ok Γ -> Γ ⊢t (random_inhabitant τ) ⋮t ⌊τ⌋.
+Proof.
+  induction τ; simpl; intros; auto.
+  - destruct B; auto.
+  - basic_typing_solver6.
+  - basic_typing_solver6.
+Qed.
+
+Global Hint Resolve random_inhabitant_tyable: core.
+
+Lemma random_inhabitant_lc: forall τ, lc (random_inhabitant τ).
+Proof.
+  intros.
+  assert ([] ⊢t (random_inhabitant τ) ⋮t ⌊τ⌋);
+  basic_typing_solver6.
+Qed.
+
+Global Hint Resolve random_inhabitant_lc: core.
+
+Ltac refinement_solver4 :=
+  repeat (match goal with
+          | [H: closed_rty _ _ _ |- lc_rty_idx _ _] => invclear H; mydestr; auto
+          | [H: closed_rty _ _ _ |- context [rty_fv _]] => invclear H; mydestr; auto
+          end || refinement_solver3).
+
+Lemma value_reduce_to_value_implies_same: forall (v1 v2: value), v1 ↪* v2 <-> v1 = v2 /\ lc v2.
+Proof.
+  split; intros.
+  - invclear H; auto. invclear H0.
+  - mydestr; subst. apply multistep_refl; auto.
+Qed.
+
+Ltac lc_solver3 :=
+  lc_solver ||
+  match goal with
+  | [|- lc (tvalue (value_msubst _ _))] =>
+      eapply instantiation_implies_value_msubst_lc; eauto;
+      basic_typing_solver
+  end.
+
+Ltac op_solver1 :=
+  op_simpl;
+  auto;
+  repeat match goal with
+    | [H: _ ⊢t ?e ⋮t _ |- lc ?e ] => apply basic_typing_regular_tm in H; destruct H; auto
+    | [H: _ ↪* ?e |- lc ?e] => apply multi_step_regular in H; mydestr; auto
+    | [H: ?Γ ⊢t ?e ⋮t ?T |- (?Γ ++ _) ⊢t ?e ⋮t _] => apply basic_typing_weaken_tm_pre; eauto
+    | [H: ?Γ ⊢t _ ⋮t _ |- ok _ ] => apply basic_typing_regular_tm in H; destruct H
+    end; listctx_set_solver.
+
+Ltac reduction_simpl1 :=
+  repeat (simpl; msubst_simpl ||
+            match goal with
+            | [H: (tvalue _) ↪* (tvalue _) |- _ ] =>
+                rewrite value_reduce_to_value_implies_same in H; mydestr; subst
+            | [|- (tvalue _) ↪* (tvalue _)] =>
+                rewrite value_reduce_to_value_implies_same; split; eauto
+            | [H: context [?e ^v^ _] |- _ ] =>
+               assert (lc e) as Htmp by (auto; lc_solver3);
+               rewrite (open_rec_lc_value _ e) in H; auto;
+               try clear Htmp
+           | [|- context [?e ^v^ _] ] =>
+               assert (lc e) as Htmp by (auto; lc_solver3);
+               rewrite (open_rec_lc_value _ e); auto;
+               try clear Htmp
+           | [H: context [?e ^t^ _] |- _ ] =>
+               assert (lc e) as Htmp by (auto; lc_solver3);
+               rewrite (open_rec_lc_tm _ e) in H; auto;
+               try clear Htmp
+           | [|- context [?e ^t^ _] ] =>
+               assert (lc e) as Htmp by (auto; lc_solver3);
+               rewrite (open_rec_lc_tm _ e); auto;
+               try clear Htmp
+            end || auto_reduction_exfalso).
+
+Lemma body_vbvar_0: body (vbvar 0).
+Proof.
+  unfold body. exists ∅. intros. constructor.
+Qed.
+
+Global Hint Resolve body_vbvar_0: core.
+
+Lemma lc_tletapp: forall (v x: value), lc v -> lc x -> lc (tletapp v x (vbvar 0)).
+Proof.
+  intros. auto_exists_L; simpl; intros; auto.
+Qed.
+
+Global Hint Resolve lc_tletapp: core.
+
+Lemma body_tletapp_0: forall (v: value), lc v -> body (tletapp v (vbvar 0) (vbvar 0)).
+Proof.
+  intros. auto_exists_L; intros. simpl. reduction_simpl1.
+Qed.
+
+Global Hint Resolve body_tletapp_0: core.
+
+Global Hint Resolve mk_app_body: core.
+
+Ltac reduction_solver1 :=
+  reduction_simpl1; eauto;
+  repeat (
+      (match goal with
+       | [|- lc (tvalue (value_msubst _ _))] =>
+           eapply instantiation_implies_value_msubst_lc; eauto;
+           basic_typing_solver6
+       | [|- lc (tm_msubst _ _)] =>
+           eapply instantiation_implies_msubst_lc; eauto;
+           basic_typing_solver6
+       end) || op_solver1 || basic_typing_solver6).
+
+Lemma tm_open_then_msubst: forall Γ env,
+    instantiation Γ env ->
+    (forall e v, tm_msubst env (e ^t^ v) = (tm_msubst env e ^t^ value_msubst env v)).
+Proof.
+  intros Γ env Hi; induction Hi; simpl; intros; auto.
+  rewrite subst_open_tm; basic_typing_solver6.
+Qed.
+
+Lemma value_open_then_msubst: forall Γ env,
+    instantiation Γ env ->
+    (forall e v, value_msubst env (e ^v^ v) = (value_msubst env e ^v^ value_msubst env v)).
+Proof.
+  intros Γ env Hi; induction Hi; simpl; intros; auto.
+  rewrite subst_open_value; basic_typing_solver6.
+Qed.
+
+Lemma mk_app_reduce_to_open:
+  ∀ (Γ : listctx ty) (Tx T : ty) e1 (v2 : value),
+    Γ ⊢t v2 ⋮v Tx -> Γ ⊢t (vlam Tx e1) ⋮v (Tx ⤍ T) ->
+    (mk_app (vlam Tx e1) v2) <-<{ Γ; T} (e1 ^t^ v2).
+Proof.
+  intros. constructor.
+  - eapply mk_app_typable; eauto.
+  - basic_typing_solver6.
+  - unfold termRraw. intros. unfold mk_app in H2. reduction_simpl1.
+    rewrite lete_step_spec in H2; simpl; mydestr. simpl in H4.
+    rewrite lete_step_spec in H4; simpl; mydestr. simpl in H6.
+    reduction_simpl1.
+    rewrite letapp_step_spec in H6; mydestr.
+    destruct H9; mydestr; invclear H9.
+    rewrite lete_step_spec in H10; simpl; mydestr. simpl in H11.
+    reduction_simpl1.
+    erewrite tm_open_then_msubst; eauto.
+Qed.
+
+Lemma body_tm_open_1_same: forall e v, body e -> {1 ~t> v} e = e.
+Proof.
+  intros. invclear H. auto_pose_fv y. specialize_with y.
+  apply fact1_tm with (j := 0) (v:=y); try lia.
+  rewrite open_rec_lc_tm; auto.
+Qed.
+
+Lemma body_value_open_1_same: forall (e: value) v, body e -> {1 ~v> v} e = e.
+Proof.
+  intros. invclear H. auto_pose_fv y. specialize_with y.
+  apply fact1_value with (j := 0) (v:=y); try lia.
+  rewrite open_rec_lc_value; auto.
+Qed.
+
+Lemma mk_app_reduce_to_let':
+  ∀ (Γ : listctx ty) (Tx T : ty) e1 e2,
+    Γ ⊢t e2 ⋮t Tx -> Γ ⊢t (vlam Tx e1) ⋮v (Tx ⤍ T) ->
+    (tlete e2 e1) <-<{ Γ; T} (mk_app (vlam Tx e1) e2).
+Proof.
+  intros. constructor; basic_typing_solver6.
+  - invclear H0. auto_exists_L; simpl; intros.
+  - eapply mk_app_typable; eauto.
+  - unfold termRraw. intros. unfold mk_app. reduction_simpl1.
+    assert (lc (tm_msubst env e2)) by reduction_solver1.
+    assert (lc (value_msubst env (vlam Tx e1))) by
+      (eapply instantiation_implies_value_msubst_lc; eauto; basic_typing_solver6).
+    rewrite lete_step_spec. split; auto.
+    eexists; split; reduction_simpl1.
+    rewrite lete_step_spec. split; auto.
+    rewrite lete_step_spec in H2; mydestr; subst.
+    eexists; split; eauto.
+    simpl. rewrite body_tm_open_1_same; reduction_solver1.
+    rewrite letapp_step_spec. repeat split; reduction_solver1.
+    left. do 2 eexists. split; auto.
+    rewrite lete_step_spec. split; auto.
+    eexists; split; reduction_solver1.
+Qed.
+
+Lemma mk_app_reduce_to_open':
+  ∀ (Γ : listctx ty) (Tx T : ty) e1 (v2 : value),
+    Γ ⊢t v2 ⋮v Tx -> Γ ⊢t (vlam Tx e1) ⋮v (Tx ⤍ T) ->
+    (e1 ^t^ v2) <-<{ Γ; T} (mk_app (vlam Tx e1) v2).
+Proof.
+  intros. constructor; basic_typing_solver6.
+  - eapply mk_app_typable; eauto.
+  - unfold termRraw. intros. unfold mk_app. reduction_simpl1.
+    assert (lc (value_msubst env v2)) by reduction_solver1.
+    assert (lc (value_msubst env (vlam Tx e1))) by
+      (eapply instantiation_implies_value_msubst_lc; eauto; basic_typing_solver6).
+    rewrite lete_step_spec. split; auto.
+    eexists; split; reduction_simpl1.
+    rewrite lete_step_spec. split; auto.
+    eexists; split; reduction_simpl1.
+    simpl. rewrite body_tm_open_1_same; reduction_solver1.
+    rewrite letapp_step_spec. repeat split; reduction_solver1.
+    left. do 2 eexists. split; auto.
+    rewrite lete_step_spec. split; auto.
+    eexists; split; reduction_solver1.
+    erewrite tm_open_then_msubst in H2; eauto.
+Qed.
+
+Ltac neg_apply H := pbc; apply H; clear H; neg_simpl.
+
+Lemma inhabitant_in_arr_rty_halt: forall τ,
+    valid_rty τ ->
+    (forall n bst st, (∀ e, ({n;bst;st}⟦τ⟧) e -> (exists v, e ↪* v)) \/ (({n;bst;st}⟦τ⟧) terr)).
+Proof.
+  intros τ Hv. induction Hv; intros.
+  - left. intros. invclear H0; mydestr; subst. eexists; eauto.
+  - destruct (classic (({n0;bst;st}⟦[v:B|n|d|ϕ]⟧) terr)); auto. left; intros.
+    neg_apply H0. invclear H1; mydestr. do 2 (split; auto). intros.
+    apply H3 in H5; auto. exfalso; auto. eapply H2; eauto.
+  - destruct (classic (({n0;bst;st}⟦-:{v: B | n | d | ϕ}⤑ τ⟧) terr)); auto. left; intros.
+    neg_apply H1. invclear H2; mydestr. do 2 (split; auto). intros.
+    apply H4 in H6; auto. eapply termR_perserve_rR; eauto. admit.
+    (* specialize (IHHv (S n0) (<b[↦c_x]> bst) st). destruct IHHv. *)
+    (* + apply H7 in H6. admit. *)
+    (* + eapply termR_perserve_rR; eauto. admit. *)
+  - destruct (classic ( ({n0;bst;st}⟦(-:{v: B | n | d | ϕ}⤑ τ1) ⤑ τ2⟧) terr)); auto. left; intros.
+    neg_apply H0. invclear H1; mydestr. do 2 (split; auto). intros.
+    apply H3 in H4; auto.
+    eapply termR_perserve_rR; eauto. admit.
+  - destruct (classic ( {n;bst;st}⟦(τ11 ⤑ τ12) ⤑ τ2⟧ terr )); auto. left; intros.
+    neg_apply H0. invclear H1; mydestr. do 2 (split; auto). intros.
+    apply H3 in H4; auto. admit.
 Admitted.
-
-Lemma rRctx_backward_under: forall Γ z τ_z (e: tm) τ,
-    ~ not_overbasety τ_z ->
-    ⟦ τ ⟧{ Γ ++ [(z, τ_z)] } e <->
-      (∃ (u_hat: tm), ⟦ τ_z ⟧{ Γ } u_hat /\
-                        (forall (u: tm), ⟦ τ_z ⟧{ Γ } u ->
-                                    (∀ (v_u: value), u_hat ↪* v_u -> ⟦ { z:= v_u }r τ ⟧{ Γ } (tlete u (e ^t^ z)))
-                        )).
-Admitted.
-
-(* Lemma no_halting_term_is_inhabitant: forall τ (st: state) n bst e, *)
-(*     not_overbasety τ -> *)
-(*     closed_rty n (dom aset st) τ -> *)
-(*     (∀ (v: value), ~ e ↪* v) -> [] ⊢t e ⋮t ⌊ τ ⌋ -> {n;bst;st}⟦τ⟧ e. *)
-(* Proof. *)
-(*   induction τ; simpl; intros. *)
-(*   - invclear H. *)
-(*   - constructor; auto. constructor; auto. intros. *)
-(*   intros. *)
-
-Inductive ctxrR_halt: state -> listctx rty -> rty -> tm -> Prop :=
-| ctxrR_halt_nil: forall st τ e, { st }⟦ τ ⟧ e -> ctxrR_halt st [] τ e
-| ctxrR_halt_cons_over: forall st (x: atom) B n d ϕ Γ τ (e: tm),
-    closed_rty 0 ({[x]} ∪ ctxdom Γ ∪ (dom _ st)) τ ->
-    ok_dctx (dom _ st) ((x, {v: B | n | d | ϕ}) :: Γ) ->
-    ((x, TBase B) :: (⌊Γ⌋*)) ⊢t e ⋮t ⌊τ⌋ ->
-     (forall (c_x: constant), {st}⟦ {v: B | n | d | ϕ} ⟧ c_x ->
-                         ctxrR_halt  (<[ x := c_x ]> st) Γ τ (tlete c_x ({ 0 <t~ x} e))) ->
-     ctxrR_halt st ((x, {v: B | n | d | ϕ}) :: Γ) τ e
-| ctxrR_halt_cons_under: forall st (x: atom) τ_x τ Γ e,
-    not_overbasety τ_x ->
-    closed_rty 0 ({[x]} ∪ ctxdom Γ ∪ (dom _ st)) τ ->
-    ok_dctx (dom _ st) ((x, τ_x) :: Γ) ->
-    ((x, ⌊τ_x⌋ ) :: (⌊Γ⌋*)) ⊢t e ⋮t ⌊τ⌋ ->
-     (exists e_x_hat, {st}⟦ τ_x ⟧ e_x_hat /\
-                   (∃ (v_x_hat: value), e_x_hat ↪* v_x_hat) /\
-                   (forall e_x, {st}⟦ τ_x ⟧ e_x ->
-                           (∀ (v_x: value), e_x_hat ↪* v_x ->
-                                            ctxrR_halt ({ x ↦ v_x } st) Γ τ (tlete e_x ({ 0 <t~ x} e))))) ->
-     ctxrR_halt  st ((x, τ_x) :: Γ) τ e.
-
-Inductive halt_ctx: state -> listctx rty -> Prop :=
-| halt_ctx_nil: ∀ st, halt_ctx st []
-| halt_ctx_cons_ubase: forall st Γ x b n d ϕ,
-    halt_ctx st Γ ->
-    ~ ({st}⟦ [v: b | n | d | ϕ ] ⟧{ Γ } terr) ->
-    halt_ctx st (Γ ++ [(x, [v: b | n | d | ϕ ])])
-| halt_ctx_cons: forall st Γ x τ,
-    not_underbasety τ ->
-    halt_ctx st Γ ->
-    halt_ctx st (Γ ++ [(x, τ)]).
-
-Inductive halt_ctx_rev: state -> listctx rty -> Prop :=
-| halt_ctx_rev_nil: ∀ st, halt_ctx_rev st []
-| halt_ctx_rev_cons_obase: forall st Γ x (b: base_ty) n d (ϕ: refinement),
-    (forall (c: constant), [] ⊢t c ⋮v b -> ϕ b∅ ∅ c -> halt_ctx_rev ({ x ↦ c } st) Γ) ->
-    halt_ctx_rev st ((x, {v: b | n | d | ϕ }) :: Γ)
-| halt_ctx_rev_cons_ubase: forall st Γ x (b: base_ty) n d (ϕ: refinement),
-    (exists (c: constant), ϕ b∅ ∅ c) ->
-    (forall (c: constant), [] ⊢t c ⋮v b -> halt_ctx_rev ({ x ↦ c } st) Γ) ->
-    halt_ctx_rev st ((x, [v: b | n | d | ϕ ]) :: Γ)
-| halt_ctx_rev_cons_arr: forall st Γ x τ,
-    is_arr τ -> halt_ctx_rev st Γ -> halt_ctx_rev st ((x, τ) :: Γ).
-
-Lemma halt_ctx_pre_destruct: forall Γ x b n d ϕ st,
-    halt_ctx st ((x, [v: b | n | d | ϕ ]) :: Γ) <->
-      (exists (c: constant), ϕ b∅ ∅ c) /\ (forall (c: constant), [] ⊢t c ⋮v b -> halt_ctx ({ x ↦ c } st) Γ).
-Proof.
-  apply (rev_ind (fun Γ => forall x b n d ϕ st,
-                      halt_ctx st ((x, [v: b | n | d | ϕ ]) :: Γ) <->
-                        (exists (c: constant), ϕ b∅ ∅ c) /\ (forall (c: constant), [] ⊢t c ⋮v b -> halt_ctx ({ x ↦ c } st) Γ)));
-  repeat split; simpl; intros.
-  - invclear H. admit. admit.
-  - constructor.
-  - mydestr. rewrite <- app_nil_l. constructor. constructor. admit.
-  - invclear H0.
-    + rewrite app_comm_cons in H1. apply app_inj_tail in H1. mydestr. invclear H1.
-      apply H in H2. mydestr. exists x. auto.
-    + rewrite app_comm_cons in H1. apply app_inj_tail in H1. mydestr. invclear H1.
-      apply H in H4. mydestr. exists x. auto.
-  - admit.
-  - mydestr. rewrite app_comm_cons. destruct (classic (not_underbasety r)).
-    + apply halt_ctx_cons; auto. rewrite H. split. exists x; auto. intros. apply H1 in H3. simpl. invclear H3.
-
-Lemma halt_ctx_implies_halt_ctx_rev: forall Γ, halt_ctx Γ -> halt_ctx_rev ∅ Γ.
-Proof.
-  induction Γ; intros.
-  - constructor.
-  - mydestr. invclear H.
-
-Lemma halt_ctx_plus_ctxrR_implies_ctxrR_halt: forall Γ τ e, halt_ctx Γ -> ⟦ τ ⟧{ Γ } e -> ctxrR_halt ∅ Γ τ e.
-Proof.
-  induction Γ; intros.
-  - invclear H0. constructor; auto.
-  - mydestr. invclear H.
 
 Lemma random_inhabitant_in_any_under: ∀ (τ: rty) (bst : bstate) n st,
     not_overbasety τ ->
@@ -589,283 +478,453 @@ Lemma random_inhabitant_in_any_under: ∀ (τ: rty) (bst : bstate) n st,
 Proof.
   induction τ; intros; invclear H; mydestr.
   - destruct B.
-    + split; simpl; auto. admit. split; auto. intros. admit.
-    + split; simpl; auto. apply mk_bool_gen_typable; auto. split; auto. intros. destruct c; invclear H.
+    + do 2 (split; simpl; auto).
+      intros. destruct c; invclear H.
+      apply mk_nat_gen_reduce_to_all_nat.
+    + do 2 (split; simpl; auto).
+      intros. destruct c; invclear H.
       apply mk_bool_gen_reduce_to_all_bool.
-  - denotation_simp. constructor; auto. admit. constructor; auto.
-    intros.
-    apply (termR_perserve_rR _ (random_inhabitant τ)); auto; try refinement_solver1. admit.
-    apply IHτ; refinement_solver1.
-  - denotation_simp. constructor; auto. admit. constructor; auto.
-    intros.
-    assert (exists (v_x: value), e_x ↪* v_x). admit. destruct H1.
-    apply (termR_perserve_rR _ (random_inhabitant τ2)); auto; try refinement_solver1. admit.
-    apply IHτ2; refinement_solver1.
+  - denotation_simp. repeat split; refinement_solver4.
+    + basic_typing_solver6.
+    + intros.
+      apply termR_perserve_rR with (e:= (random_inhabitant τ)); refinement_solver4.
+      assert
+        ((random_inhabitant τ ^t^ c_x) <-<{ []; ⌊τ⌋} (mk_app (vlam B (random_inhabitant τ)) c_x)). apply mk_app_reduce_to_open'; auto; basic_typing_solver6.
+      reduction_simpl1.
+      apply IHτ; refinement_solver4.
+  - denotation_simp. repeat split; refinement_solver4.
+    + basic_typing_solver6.
+    + intros.
+      (* assert (closed_rty n (dom aset st) τ1) by refinement_solver4. *)
+      assert (closed_rty n (dom aset st) τ2) by refinement_solver4.
+      (* assert (not_overbasety τ1) by (invclear H0; invclear H3; simpl; auto). *)
+      assert (not_overbasety τ2) by (invclear H0; invclear H2; simpl; auto).
+      (* apply IHτ1 with (bst:=bst) in H1; auto. *)
+      apply IHτ2 with (bst:=bst) in H1; auto.
+      apply termR_perserve_rR with (e:= tlete e_x (random_inhabitant τ2)); refinement_solver4.
+      apply mk_app_reduce_to_let'; auto; refinement_solver4; basic_typing_solver6.
+      apply termR_perserve_rR with (e:= random_inhabitant τ2); refinement_solver4.
+      admit.
 Admitted.
 
-Lemma denotation_weaken_empty: forall Γ (e: tm) τ (st: state),
+Lemma rRctx_last_underbase_not_err_implies_drop: forall Γ st τ x b n d ϕ e,
     not_overbasety τ ->
-    valid_rty τ ->
-    ok_dctx (dom _ st) Γ -> { st }⟦ τ ⟧ e -> {st}⟦ τ ⟧{ Γ } e.
+    ¬ ({st}⟦[v:b|n|d|ϕ]⟧{Γ} terr) ->
+    ok_dctx (dom _ st) (Γ ++ [(x, [v:b|n|d|ϕ])]) ->
+    (* closed_rty 0 (ctxdom Γ ∪ (dom _ st)) τ -> *)
+    {st}⟦τ⟧{Γ} e -> {st}⟦τ⟧{Γ ++ [(x, [v:b|n|d|ϕ])] } e.
 Proof.
-  induction Γ; intros; denotation_simp; mydestr.
-  constructor; auto.
-  destruct (classic (not_overbasety r)).
-  - constructor; auto; try refinement_solver1.
-    exists (random_inhabitant r); invclear H1;
-    assert (({0;b∅;st}⟦r⟧) (random_inhabitant r)) by
-      (intros; apply random_inhabitant_in_any_under; auto);
-    split; try (apply random_inhabitant_in_any_under; auto); intros.
-    + assert ([] ⊢t v_x ⋮v ⌊r⌋) as Hv_x by refinement_solver1.
-      destruct v_x; mydestr; simpl; try auto_ty_exfalso.
-      apply (termR_perserve_ctxrR _ _ e); auto. admit.
-      apply IHΓ; auto. denotation_simp. intros. rewrite rR_shadow_update_st; auto; refinement_solver1.
-      apply rR_regular1 in H2; mydestr. refinement_solver1.
-    + apply (termR_perserve_ctxrR _ _ e); auto. admit.
-      apply IHΓ; auto. denotation_simp. admit. admit.
-  - refinement_solver1. constructor; auto; try refinement_solver1.
-    intros. apply (termR_perserve_ctxrR _ _ e); auto. admit.
-    invclear H1; apply IHΓ; auto; try auto_ty_exfalso; try ok_dctx_solver_slow.
-    intros. rewrite rR_shadow_update_st; auto; refinement_solver1.
-    apply rR_regular1 in H2; mydestr. refinement_solver1.
+  induction Γ; simpl; intros; auto.
+  - constructor.
+    + refinement_solver.
+    + denotation_simp; refinement_solver.
+    + RD_simp; denotation_simp; refinement_solver.
+    + RD_simp; denotation_simp; refinement_solver.
+    + exists (random_inhabitant [v:b|n|d|ϕ]). split. admit.
+      intros. RD_simp. admit.
+  - invclear H2.
+    + constructor; auto; refinement_solver. admit. admit.
+      intros. apply H11 in H2.
+      apply IHΓ; auto. admit. admit.
+    + mydestr. constructor; auto; refinement_solver. admit. admit.
+      exists x1. split; auto. intros.
+      eapply H3 in H4; eauto.
+      apply IHΓ; auto. admit. admit.
 Admitted.
 
-Lemma denotation_weaken: forall Γ1 Γ3 (e: tm) τ (st: state) Γ2,
-    ctxrR_wf (dom _ st) (Γ1 ++ Γ2 ++ Γ3) τ -> {st}⟦ τ ⟧{ Γ1 ++ Γ3 } e -> {st}⟦ τ ⟧{ Γ1 ++ Γ2 ++ Γ3 } e.
+Lemma rRctx_last_not_underbase_implies_drop: forall Γ st τ x r e,
+    not_overbasety τ ->
+    not_underbasety r ->
+    ok_dctx (dom _ st) (Γ ++ [(x, r)]) ->
+    {st}⟦τ⟧{Γ} e -> {st}⟦τ⟧{Γ ++ [(x, r)] } e.
 Proof.
-  intros. generalize dependent Γ2.
-  induction H0; intros; listctx_set_simpl.
-  - specialize (H b∅). invclear H; mydestr. denotation_simp.
-  induction Γ1; intros; listctx_set_simpl.
-  - admit.
-  - 
-
-Lemma err_exists_denotation_excluded: forall Γ b n (d: aset) (ϕ: refinement),
-    closed_rty 0 (dom aset (∅: state)) [v:b|n|d|ϕ] ->
-    ~ (⟦ [v: b | n | d | ϕ ] ⟧{ Γ } terr) -> (∃ (v: value), ⟦ {v: b | n | d | ϕ } ⟧{ Γ } v).
-Proof.
-  induction Γ; intros.
-  - destruct (classic (∃ v : value, (⟦{v:b|n|d|ϕ}⟧{ [] }) v)); auto; exfalso; apply H0; clear H0.
-    rewrite forall_iff_not_exists1 in H1.
-    constructor. intros.
-    do 2 constructor; auto. rewrite terr_reduction_iff_false_phi.
-    intros. intros Hf.
-    specialize (H1 c). apply H1.
-    constructor; auto. intros. constructor; auto. constructor; auto.
-    rewrite closed_rty_under_iff_over; auto.
-    exists c. constructor; auto. constructor; auto.
-    rewrite bound_in_refinement_0. apply Hf. refinement_solver1.
-  - mydestr. refinement_simp1.
-    destruct (classic (∃ v : value, (⟦{v:b|n|d|ϕ}⟧{ a :: Γ }) v)); auto; exfalso; apply H0; clear H0.
-    rewrite forall_iff_not_exists1 in H1.
-    mydestr.
-    constructor.
-
-
-    repeat match goal with
-           | [H: closed_rty _ _ _ |- bound_in_refinement _ _ ] => destruct H; mydestr
-           | [H: valid_rty _ |- bound_in_refinement _ _ ] => invclear H
-           | [H: wf_r _ _ ?ϕ |- bound_in_refinement _ ?ϕ ] =>  destruct H
-           end.
-    refinement_simp1; auto.
-    repeat match goal with
-    | [H: lc_rty_idx 0 [v:_|?n|_|_] |- _ ] =>
-        match n with
-        | 0 => fail 1
-        | _ =>  assert (n = 0) by (apply lc_rty_idx_under_0_is_0 in H; auto); subst
-        end
-    end.
-    repeat match goal with
-           | [H: closed_rty _ _ _ |- bound_in_refinement _ _ ] => destruct H; mydestr
-           | [H: valid_rty _ |- bound_in_refinement _ _ ] => invclear H
-           | [H: wf_r _ _ ?ϕ |- bound_in_refinement _ ?ϕ ] =>  destruct H
-           end.
-    assert (n = 0) by (apply lc_rty_idx_under_0_is_0 in H2; auto); subst.
-    invclear H2.
-    destruct H5. 
-    invclear H.
- mydestr. invclear H. invclear H6. unfold bound_in_refinement in H5.
-    assert (closed_rty 0 ∅ [v:b|n|d|ϕ]). setoid_rewrite <- H2; auto.
-
-    setoid_rewrite H2 in H.
-
-    admit. auto.
-    intros. apply multistep_R.
-
-    constructor.
-    exfalso. apply H. constructor; intros. rewrite terr_inhabitant_iff_false_phi.
-
-
-  intros. destruct (classic (∃ v : value, (⟦[v:b|n|d|ϕ]⟧{Γ}) v)); auto.
-  exfalso. apply H. rewrite terr_inhabitant_iff_false_phi.
-
-  intro Hf. mydestr. invclear Hf.
-    + invclear H. denotation_simp.
-      match goal with
-      | [H: ∀ c, [] ⊢t (vconst c) ⋮v _ → _ _ ∅ c → terr ↪* (tvalue (vconst c)) |- _ ] => idtac H
-      end.
-      rewrite terr_inhabitant_implies_false_phi in H4.
-      apply H4 in H7.
-      repeat match goal with
-      | [H: _ ⊢t ?v ⋮v (TBase _) |- _ ] =>
-          match v with
-          | vconst _ => fail 1
-          | _ => set H7 as Htmp; apply empty_basic_typing_base_const_exists in Htmp; mydestr; subst
-          end
-      end.
-      set H7 as Htmp; apply empty_basic_typing_base_const_exists in Htmp; mydestr; subst.
-      match goal with
-      | [H: _ ⊢t (tvalue ?v) ⋮t _ |- _ ] => invclear H
-      end.
-
-      apply empty_basic_typing_base_const_exists in H.
-
-       specialize (H1 b∅).
-      invclear H0. invclear H1. mydestr.
+  induction Γ; simpl; intros; auto.
+  - destruct (classic (not_overbasety r)).
+    + constructor; auto.
+      { denotation_simp; refinement_solver. }
+      { RD_simp; denotation_simp; refinement_solver. }
+      exists (random_inhabitant r). split. admit.
+      intros. RD_simp. admit.
+    + refinement_simp1. RD_simp. constructor; auto.
+      { denotation_simp; refinement_solver. }
+      { RD_simp; denotation_simp; refinement_solver. }
+      intros. constructor. admit.
+  - invclear H2.
+    + constructor; auto; refinement_solver. admit. admit.
+      intros. apply H11 in H2.
+      apply IHΓ; auto. admit.
+    + mydestr. constructor; auto; refinement_solver. admit. admit.
+      exists x1. split; auto. intros.
+      eapply H3 in H4; eauto.
+      apply IHΓ; auto. admit.
 Admitted.
 
-(* Denotation: *)
-
-Fixpoint rR (n: nat) (bst: bstate) (st: state) (τ: rty) (e: tm) : Prop :=
-  [] ⊢t e ⋮t ⌊ τ ⌋ /\ closed_rty n (dom _ st) τ /\
-    match τ with
-    | {v: B | _ | _ | ϕ} => exists (c: constant), [] ⊢t c ⋮v B /\ ϕ bst st c /\ e = c
-    | [v: B | _ | _ | ϕ] => forall (c: constant), [] ⊢t c ⋮v B -> ϕ bst st c -> e ↪* c
-    | -:{v: B | _ | _ | ϕ } ⤑ τ =>
-        forall (c_x: constant), [] ⊢t c_x ⋮v B -> ϕ bst st c_x -> rR (S n) (<b[↦ c_x ]> bst) st τ (mk_app e c_x)
-    | τ1 ⤑ τ2 => forall (e_x: tm), rR n bst st τ1 e_x -> rR n bst st τ2 (mk_app e e_x)
-    end.
-
-Notation " '{' n ';' bst ';' st '}⟦' τ '⟧' " :=
-  (rR n bst st τ) (at level 20, format "{ n ; bst ; st }⟦ τ ⟧", bst constr, st constr, τ constr).
-Notation " '{' st '}⟦' τ '⟧' " := (fun e => forall bst, rR 0 bst st τ e) (at level 20, format "{ st }⟦ τ ⟧", st constr, τ constr).
-Notation " '⟦' τ '⟧' " := (fun e => forall bst, rR 0 bst ∅ τ e) (at level 20, format "⟦ τ ⟧", τ constr).
-
-(* regular of the denation *)
-
-Lemma rR_regular1:
-  forall τ n bst st e, { n; bst; st }⟦ τ ⟧ e -> closed_rty n (dom _ st) τ /\ [] ⊢t e ⋮t ⌊ τ ⌋.
+Lemma rRctx_pre_weakening: forall Γ2 Γ1 τ,
+    not_overbasety τ ->
+    (Γ1 ++ Γ2) ⊢WF τ -> (forall e, ⟦τ⟧{Γ1} e -> ⟦τ⟧{Γ1 ++ Γ2} e).
 Proof.
-  induction τ; intros; invclear H; mydestr; subst; split; intros; auto.
-Qed.
+  apply (rev_ind (fun Γ2 => forall Γ1 τ,
+                      not_overbasety τ ->
+                      (Γ1 ++ Γ2) ⊢WF τ -> (forall e, ⟦τ⟧{Γ1} e -> ⟦τ⟧{Γ1 ++ Γ2} e)));
+    intros; denotation_simp; auto.
+  - invclear H1. invclear H3; listctx_set_simpl. admit. admit.
+Admitted.
 
-Lemma rR_regular2:
-  forall τ st e, { st }⟦ τ ⟧ e -> closed_rty 0 (dom _ st) τ /\ [] ⊢t e ⋮t ⌊ τ ⌋.
-Proof.
-  intros. specialize (H b∅). eapply rR_regular1; eauto.
-Qed.
+Lemma rRctx_weakening_empty: forall Γ τ, Γ ⊢WF τ -> (forall e, ⟦τ⟧ e -> ⟦τ⟧{Γ} e).
+Admitted.
 
-Lemma rR_regular3:
-  forall τ e, ⟦ τ ⟧ e -> (closed_rty 0 ∅ τ) /\ [] ⊢t e ⋮t ⌊ τ ⌋.
-Proof.
-  intros. eapply rR_regular2 in H. mydestr; split; auto.
-  intros. apply H. my_set_solver.
-Qed.
-
-Inductive ctxrR_wf: aset -> listctx rty -> rty -> Prop :=
-| ctxrR_wf_nil: forall d τ, closed_rty 0 d τ -> ctxrR_wf d [] τ
-| ctxrR_wf_cons_over: forall d (x: atom) τ_x Γ τ,
-    ok_dctx d ((x, τ_x) :: Γ) ->
-    closed_rty 0 d τ_x ->
-    ctxrR_wf ({[x]} ∪ d) Γ τ ->
-    ctxrR_wf d ((x, τ_x) :: Γ) τ.
-
-Inductive ctxrR: state -> listctx rty -> rty -> tm -> Prop :=
-| ctxrR_nil: forall st τ e, { st }⟦ τ ⟧ e -> ctxrR st [] τ e
-| ctxrR_cons_over: forall st (x: atom) B d ϕ Γ τ (e: tm),
-    ctxrR_wf (dom _ st) ((x, {v: B | 0 | d | ϕ}) :: Γ) τ ->
-    ((x, TBase B) :: (⌊Γ⌋*)) ⊢t e ⋮t ⌊τ⌋ ->
-     (forall (c_x: constant), {st}⟦ {v: B | 0 | d | ϕ} ⟧ c_x ->
-                         ctxrR (<[ x := c_x ]> st) Γ τ (tlete c_x ({ 0 <t~ x} e))) ->
-     ctxrR st ((x, {v: B | 0 | d | ϕ}) :: Γ) τ e
-| ctxrR_cons_under: forall st (x: atom) τ_x τ Γ e,
-        ctxrR_wf (dom _ st) ((x, τ_x) :: Γ) τ ->
-        ((x, ⌊τ_x⌋ ) :: (⌊Γ⌋*)) ⊢t e ⋮t ⌊τ⌋ ->
-         not_overbasety τ_x ->
-         (exists e_x_hat, {st}⟦ τ_x ⟧ e_x_hat /\
-                       (forall e_x, {st}⟦ τ_x ⟧ e_x ->
-                               (∀ (v_x: value), e_x_hat ↪* v_x ->
-                                                ctxrR ({ x ↦ v_x } st) Γ τ (tlete e_x ({ 0 <t~ x} e))))) ->
-         ctxrR st ((x, τ_x) :: Γ) τ e.
-
-Notation " '{' st '}⟦' τ '⟧{' Γ '}' " := (ctxrR st Γ τ) (at level 20, format "{ st }⟦ τ ⟧{ Γ }", st constr, τ constr, Γ constr).
-Notation " '⟦' τ '⟧{' Γ '}' " := (ctxrR ∅ Γ τ) (at level 20, format "⟦ τ ⟧{ Γ }", τ constr, Γ constr).
-
-Lemma ctxrR_implies_ctxrR_wf:
-  forall Γ τ st e, { st }⟦ τ ⟧{ Γ } e -> ctxrR_wf (dom _ st) Γ τ.
-Proof.
-  induction Γ; simpl; intros; invclear H; simpl; auto.
-  - apply rR_regular2 in H0; mydestr. constructor; auto.
-Qed.
-
-Lemma ctxrR_wf_regular:
-  forall Γ τ d, ctxrR_wf d Γ τ -> (ok_dctx d Γ) /\ cl_dctx d Γ /\ closed_rty 0 (ctxdom Γ ∪ d) τ.
-Proof.
-  induction Γ; simpl; intros; invclear H; simpl.
-  - split. repeat constructor; auto; fast_set_solver.
-    split. constructor.
-    closed_rty_solver.
-  - apply IHΓ in H6; mydestr2.
-    split; auto.
-    split. constructor; listctx_set_simpl. closed_rty_solver.
-Qed.
-
-Lemma ctxrR_regular0:
-  forall Γ τ st e, { st }⟦ τ ⟧{ Γ } e ->
-              (ok_dctx (dom _ st) Γ) /\ cl_dctx (dom _ st) Γ /\ closed_rty 0 (ctxdom Γ ∪ (dom _ st)) τ.
-Proof.
-  intros. apply ctxrR_wf_regular. eapply ctxrR_implies_ctxrR_wf; eauto.
-Qed.
-
-Lemma ctxrR_regular1:
-  forall Γ τ st e, { st }⟦ τ ⟧{ Γ } e -> ⌊ Γ ⌋* ⊢t e ⋮t ⌊ τ ⌋.
-Proof.
-  induction Γ; simpl; intros; invclear H; simpl; auto.
-  - apply rR_regular2 in H0; mydestr; auto.
-Qed.
-
-Lemma ctxrR_regular:
-  forall Γ τ st e, { st }⟦ τ ⟧{ Γ } e ->
-              ⌊ Γ ⌋* ⊢t e ⋮t ⌊ τ ⌋ /\
-                (ok_dctx (dom _ st) Γ) /\
-                cl_dctx (dom _ st) Γ /\
-                closed_rty 0 (ctxdom Γ ∪ (dom _ st)) τ.
-Proof.
-  intros. split.
-  - eapply ctxrR_regular1; eauto.
-  - eapply ctxrR_regular0; eauto.
-Qed.
-
-(* Lemma ctxrR_regular1: *)
-(*   forall Γ τ st e, { st }⟦ τ ⟧{ Γ } e -> closed_rty 0 (ctxdom Γ ∪ dom _ st) τ /\ *)
-(*                 ⌊ Γ ⌋* ⊢t e ⋮t ⌊ τ ⌋ /\ (ok_dctx (dom _ st) Γ). *)
+(* Lemma rRctx_backward_over: forall Γ z b n d ϕ (e: tm) τ, *)
+(*     not_overbasety τ -> *)
+(*     (forall st, {st}⟦ τ ⟧{ Γ ++ [(z, {v: b | n | d | ϕ})] } e) <-> *)
+(*       (forall st, *)
+(*           (closed_rty 0 (ctxdom (Γ ++ [(z, {v: b | n | d | ϕ})]) ∪ dom aset st) τ /\ *)
+(*              ok_dctx (dom aset st) (Γ ++ [(z, {v: b | n | d | ϕ})]) /\ *)
+(*              (⌊Γ ++ [(z, {v: b | n | d | ϕ})]⌋ ⊢t e ⋮t ⌊τ⌋ /\ *)
+(*                 (forall (u: constant), {st}⟦ {v: b | n | d | ϕ} ⟧{ Γ } u -> {st}⟦ { z := u }r τ ⟧{ Γ } ({ z := u }t e)))). *)
 (* Proof. *)
-(*   induction Γ; simpl; intros; invclear H; simpl. *)
-(*   - apply rR_regular2 in H0; mydestr; split; intros; my_simplify_map_eq. *)
-(*     closed_rty_solver. *)
-(*     split; auto. constructor; auto. fast_set_solver. *)
-(*   - split; auto. closed_rty_solver. *)
-(*   - mydestr. split; auto. apply rR_regular2 in H; mydestr. closed_rty_solver. *)
-(* Qed. *)
+(*   induction Γ; split; simpl; intros; denotation_simp. *)
+(*   - specialize (H0 st). RD_simp. split; denotation_simp. split; auto. split; auto. *)
+(*     intros. RD_simp. apply H13 in H1. RD_simp. *)
+(*     rewrite denotation_st_update_iff_subst in H0; mydestr; auto; refinement_solver3. *)
+(*   - specialize (H0 st); mydestr. constructor; try refinement_solver. intros. *)
+(*     assert (({st}⟦{v:b|n|d|ϕ}⟧{ [] }) c_x) as HH by (constructor; auto). *)
+(*     apply H3 in HH. RD_simp. *)
+(*     rewrite denotation_st_update_iff_subst; refinement_solver3. *)
+(*     split; refinement_solver3. *)
+(*   - specialize (H0 st). *)
+(*     assert (ok_dctx (dom aset st) ((a, r) :: Γ ++ [(z, {v:b|n|d|ϕ})])) as Hok by *)
+(*     (apply ctxrR_regular1 in H0; mydestr; auto). *)
+(*     invclear H0; denotation_simp. *)
+(*     + do 3 (split; auto). intros. invclear H0. *)
+(*       { apply ctxrR_cons_over; denotation_simp; auto. admit. admit. *)
+(*         intros. *)
+(*         assert (({<[a:=c_x]> st}⟦{v:b|0|d|ϕ}⟧{Γ}) ({a := c_x}v u)) by auto. *)
+(*         assert ({<[a:=c_x]> st}⟦τ⟧{ Γ ++ [(z, {v:b|0|d|ϕ})] } ({a := c_x}t e)) by auto. *)
+(*         rewrite IHΓ in H3; mydestr; auto. *)
+(*         apply H8 in H1. lc_simpl. rewrite subst_commute_tm; simpl; auto; refinement_solver. *)
+(*         admit. fast_set_solver. *)
+(*       } *)
+(*       { mydestr. constructor; denotation_simp; auto. } *)
+(*     + do 3 (split; auto). intros. *)
+(*       invclear H2. *)
+(*       { apply ctxrR_cons_over; denotation_simp; auto. } *)
+(*       { mydestr. constructor; denotation_simp; auto. admit. admit. *)
+(*         exists x. *)
+(*         (* assert (({0;b∅;st}⟦r⟧) (random_inhabitant r)) as Hzz. admit. *) *)
+(*         split; auto. intros. eapply H1 in H6; eauto. *)
+(*         rewrite IHΓ in H6; mydestr; auto. *)
+(*         assert (({({a↦v_x}) st}⟦{v:b|0|d|ϕ}⟧{Γ}) u) as Hu. admit. *)
+(*         apply H16 in Hu. simpl in Hu. admit. *)
+(*       } *)
+(*   - destruct (classic (not_overbasety r)). *)
+(*     + constructor; try refinement_solver3. admit. *)
+(*       (* exists (random_inhabitant r). split. admit. intros. *) *)
+(*       (* rewrite IHΓ; auto. split. admit. split. admit. split. admit. *) *)
+(*       (* intros. *) *)
+(*       (* assert (({st}⟦{v:b|n|d|ϕ}⟧{(a, r) :: Γ}) u) as Hu. *) *)
+(*       (* { constructor; auto. admit. admit. admit. admit. } *) *)
+(*       (* apply H3 in Hu. invclear Hu. denotation_simp. mydestr. *) *)
+(*     + refinement_simp1. apply ctxrR_cons_over; denotation_simp; auto. *)
+(*       intros. *)
+(*       rewrite IHΓ; auto. split. admit. split. admit. split. admit. *)
+(*       intros. *)
+(*       assert (({st}⟦{v:b|n|d|ϕ}⟧{(a, {v:x|x0|x1|x2}) :: Γ}) u) as Hu. *)
+(*       { constructor. admit. admit. admit. admit. } *)
 
-Inductive ctxrR2: bstate -> state -> listctx rty -> rty -> rty -> Prop :=
-| ctxrR2_nil: forall bst st τ1 τ2,
-    closed_rty 0 (dom _ st) τ1 -> closed_rty 0 (dom _ st) τ2 ->
-    (forall e, { st }⟦ τ1 ⟧ e -> { st }⟦ τ2 ⟧ e) ->
-    ctxrR2 bst st [] τ1 τ2
-| ctxrR2_cons_over: forall bst st (x: atom) B d ϕ Γ τ1 τ2,
-    ctxrR_wf (dom _ st) ((x, {v: B | 0 | d | ϕ}) :: Γ) τ1 ->
-    ctxrR_wf (dom _ st) ((x, {v: B | 0 | d | ϕ}) :: Γ) τ2 ->
-    (forall (c_x: constant), {st}⟦ {v: B | 0 | d | ϕ} ⟧ c_x -> ctxrR2 bst (<[ x := c_x ]> st) Γ τ1 τ2) ->
-    ctxrR2 bst st ((x, {v: B | 0 | d | ϕ}) :: Γ) τ1 τ2
-| ctxrR2_cons_under: forall bst st (x: atom) τ_x τ1 τ2 Γ,
-    ctxrR_wf (dom _ st) ((x, τ_x) :: Γ) τ1 ->
-    ctxrR_wf (dom _ st) ((x, τ_x) :: Γ) τ2 ->
-    not_overbasety τ_x ->
-    (exists e_x_hat, {st}⟦ τ_x ⟧ e_x_hat /\
-                  (forall e_x, {st}⟦ τ_x ⟧ e_x ->
-                          (∀ (v_x: value), e_x_hat ↪* v_x -> ctxrR2 bst ({ x ↦ v_x } st) Γ τ1 τ2))) ->
-    ctxrR2 bst st ((x, τ_x) :: Γ) τ1 τ2.
+(*       auto_ty_exfalso. apply ctxrR_cons_over; try refinement_solver3. *)
+(*       intros. rewrite IHΓ. split. admit. split. admit. split. admit. *)
+(*       intros. admit. *)
+(* Admitted. *)
 
-Notation " '{' st '}⟦' τ1 '⟧⊆⟦' τ2 '⟧{' Γ '}' " := (forall bst, ctxrR2 bst st Γ τ1 τ2) (at level 20, format "{ st }⟦ τ1 ⟧⊆⟦ τ2 ⟧{ Γ }", st constr, τ1 constr, τ2 constr, Γ constr).
-Notation " '⟦' τ1 '⟧⊆⟦' τ2 '⟧{' Γ '}' " := (forall bst, ctxrR2 bst ∅ Γ τ1 τ2) (at level 20, format "⟦ τ1 ⟧⊆⟦ τ2 ⟧{ Γ }", τ1 constr, τ2 constr, Γ constr).
+Lemma rRctx_backward_over_forward: forall Γ st z b n d ϕ (e: tm) τ,
+    not_overbasety τ ->
+    {st}⟦ τ ⟧{ Γ ++ [(z, {v: b | n | d | ϕ})] } e ->
+      (closed_rty 0 (ctxdom (Γ ++ [(z, {v: b | n | d | ϕ})]) ∪ dom aset st) τ /\
+         ok_dctx (dom aset st) (Γ ++ [(z, {v: b | n | d | ϕ})]) /\
+         (⌊Γ ++ [(z, {v: b | n | d | ϕ})]⌋*) ⊢t e ⋮t ⌊τ⌋ /\
+            (forall (u: constant), {st}⟦ {v: b | n | d | ϕ} ⟧{ Γ } u -> {st}⟦ { z := u }r τ ⟧{ Γ } ({ z := u }t e))).
+Proof.
+  induction Γ; simpl; intros; denotation_simp.
+  - RD_simp. split; denotation_simp. split; auto. split; auto.
+    intros. RD_simp. apply H13 in H1. RD_simp.
+    rewrite denotation_st_update_iff_subst in H0; mydestr; auto; refinement_solver3.
+  - assert (ok_dctx (dom aset st) ((a, r) :: Γ ++ [(z, {v:b|n|d|ϕ})])) as Hok by
+    (apply ctxrR_regular1 in H0; mydestr; auto).
+    invclear H0; denotation_simp.
+    + do 3 (split; auto). intros. invclear H0.
+      { apply ctxrR_cons_over; denotation_simp; auto. admit. admit.
+        intros.
+        assert (({<[a:=c_x]> st}⟦{v:b|0|d|ϕ}⟧{Γ}) ({a := c_x}v u)) by auto.
+        assert ({<[a:=c_x]> st}⟦τ⟧{ Γ ++ [(z, {v:b|0|d|ϕ})] } ({a := c_x}t e)) by auto.
+        apply IHΓ in H3; mydestr; auto.
+        apply H8 in H1. lc_simpl. rewrite subst_commute_tm; simpl; auto; refinement_solver.
+        admit. fast_set_solver.
+      }
+      { mydestr. constructor; denotation_simp; auto. }
+    + do 3 (split; auto). intros.
+      invclear H2.
+      { apply ctxrR_cons_over; denotation_simp; auto. }
+      { mydestr. constructor; denotation_simp; auto. admit. admit.
+        exists x.
+        (* assert (({0;b∅;st}⟦r⟧) (random_inhabitant r)) as Hzz. admit. *)
+        split; auto. intros. eapply H1 in H6; eauto.
+        apply IHΓ in H6; mydestr; auto.
+        assert (({({a↦v_x}) st}⟦{v:b|0|d|ϕ}⟧{Γ}) u) as Hu. admit.
+        apply H16 in Hu. simpl in Hu. admit.
+      }
+Admitted.
+
+(* Lemma rRctx_backward_over: forall Γ st z b n d ϕ (e: tm) τ, *)
+(*     not_overbasety τ -> *)
+(*     {st}⟦ τ ⟧{ Γ ++ [(z, {v: b | n | d | ϕ})] } e <-> *)
+(*       (closed_rty 0 (ctxdom (Γ ++ [(z, {v: b | n | d | ϕ})]) ∪ dom aset st) τ /\ *)
+(*          ok_dctx (dom aset st) (Γ ++ [(z, {v: b | n | d | ϕ})]) /\ *)
+(*          (⌊Γ ++ [(z, {v: b | n | d | ϕ})]⌋ ⊢t e ⋮t ⌊τ⌋ /\ *)
+(*             (forall (u: constant), {st}⟦ {v: b | n | d | ϕ} ⟧{ Γ } u -> {st}⟦ { z := u }r τ ⟧{ Γ } ({ z := u }t e))). *)
+(* Proof. *)
+(*   induction Γ; split; simpl; intros; denotation_simp. *)
+(*   - RD_simp. split; denotation_simp. split; auto. split; auto. *)
+(*     intros. RD_simp. apply H13 in H1. RD_simp. *)
+(*     rewrite denotation_st_update_iff_subst in H0; mydestr; auto; refinement_solver3. *)
+(*   - constructor; try refinement_solver. intros. *)
+(*     assert (({st}⟦{v:b|n|d|ϕ}⟧{ [] }) c_x) as HH by (constructor; auto). *)
+(*     apply H3 in HH. RD_simp. *)
+(*     rewrite denotation_st_update_iff_subst; refinement_solver3. *)
+(*     split; refinement_solver3. *)
+(*   - assert (ok_dctx (dom aset st) ((a, r) :: Γ ++ [(z, {v:b|n|d|ϕ})])) as Hok by *)
+(*     (apply ctxrR_regular1 in H0; mydestr; auto). *)
+(*     invclear H0; denotation_simp. *)
+(*     + do 3 (split; auto). intros. invclear H0. *)
+(*       { apply ctxrR_cons_over; denotation_simp; auto. admit. admit. *)
+(*         intros. *)
+(*         assert (({<[a:=c_x]> st}⟦{v:b|0|d|ϕ}⟧{Γ}) ({a := c_x}v u)) by auto. *)
+(*         assert ({<[a:=c_x]> st}⟦τ⟧{ Γ ++ [(z, {v:b|0|d|ϕ})] } ({a := c_x}t e)) by auto. *)
+(*         rewrite IHΓ in H3; mydestr; auto. *)
+(*         apply H8 in H1. lc_simpl. rewrite subst_commute_tm; simpl; auto; refinement_solver. *)
+(*         admit. fast_set_solver. *)
+(*       } *)
+(*       { mydestr. constructor; denotation_simp; auto. } *)
+(*     + do 3 (split; auto). intros. *)
+(*       invclear H2. *)
+(*       { apply ctxrR_cons_over; denotation_simp; auto. } *)
+(*       { mydestr. constructor; denotation_simp; auto. admit. admit. *)
+(*         exists x. *)
+(*         (* assert (({0;b∅;st}⟦r⟧) (random_inhabitant r)) as Hzz. admit. *) *)
+(*         split; auto. intros. eapply H1 in H6; eauto. *)
+(*         rewrite IHΓ in H6; mydestr; auto. *)
+(*         assert (({({a↦v_x}) st}⟦{v:b|0|d|ϕ}⟧{Γ}) u) as Hu. admit. *)
+(*         apply H16 in Hu. simpl in Hu. admit. *)
+(*       } *)
+(*   - destruct (classic (not_overbasety r)). *)
+(*     + constructor; try refinement_solver3. admit. *)
+(*       (* exists (random_inhabitant r). split. admit. intros. *) *)
+(*       (* rewrite IHΓ; auto. split. admit. split. admit. split. admit. *) *)
+(*       (* intros. *) *)
+(*       (* assert (({st}⟦{v:b|n|d|ϕ}⟧{(a, r) :: Γ}) u) as Hu. *) *)
+(*       (* { constructor; auto. admit. admit. admit. admit. } *) *)
+(*       (* apply H3 in Hu. invclear Hu. denotation_simp. mydestr. *) *)
+(*     + refinement_simp1. apply ctxrR_cons_over; denotation_simp; auto. *)
+(*       intros. *)
+(*       rewrite IHΓ; auto. split. admit. split. admit. split. admit. *)
+(*       intros. *)
+(*       assert (({st}⟦{v:b|n|d|ϕ}⟧{(a, {v:x|x0|x1|x2}) :: Γ}) u) as Hu. *)
+(*       { constructor. admit. admit. admit. admit. } *)
+(*       (* auto_ty_exfalso. apply ctxrR_cons_over; try refinement_solver3. *) *)
+(*       (* intros. rewrite IHΓ. split. admit. split. admit. split. admit. *) *)
+(*       (* intros. admit. *) *)
+(* Admitted. *)
+
+
+(* Lemma rRctx_backward_over: forall Γ st z b n d ϕ (e: tm) τ, *)
+(*     not_overbasety τ -> *)
+(*     {st}⟦ τ ⟧{ Γ ++ [(z, {v: b | n | d | ϕ})] } e <-> *)
+(*       (closed_rty 0 (ctxdom (Γ ++ [(z, {v: b | n | d | ϕ})]) ∪ dom aset st) τ /\ *)
+(*          ok_dctx (dom aset st) (Γ ++ [(z, {v: b | n | d | ϕ})]) /\ *)
+(*          (⌊Γ ++ [(z, {v: b | n | d | ϕ})]⌋ ⊢t e ⋮t ⌊τ⌋ /\ *)
+(*             (forall (u: value), {st}⟦ {v: b | n | d | ϕ} ⟧{ Γ } u -> {st}⟦ { z := u }r τ ⟧{ Γ } ({ z := u }t e))). *)
+(* Proof. *)
+(*   induction Γ; split; simpl; intros; denotation_simp. *)
+(*   - RD_simp. split; denotation_simp. split; auto. split; auto. *)
+(*     intros. RD_simp. apply H13 in H1. RD_simp. *)
+(*     rewrite denotation_st_update_iff_subst in H0; mydestr; auto; refinement_solver3. *)
+(*     (* eapply termR_perserve_rR; eauto; refinement_solver3. ctx_erase_simp4. *) *)
+(*     (* apply termR_let_one_step_from_basic_type; auto. *) *)
+(*     (* basic_typing_solver. refinement_solver3. refinement_solver. denotation_simp. *) *)
+(*   - constructor; try refinement_solver. intros. *)
+(*     assert (({st}⟦{v:b|n|d|ϕ}⟧{ [] }) c_x) as HH by (constructor; auto). *)
+(*     apply H3 in HH. RD_simp. *)
+(*     rewrite denotation_st_update_iff_subst; refinement_solver3. *)
+(*     split; refinement_solver3. *)
+(*     (* denotation_simp. *) *)
+(*     (* eapply termR_perserve_rR; eauto; denotation_simp; refinement_solver3. *) *)
+(*     (* apply termR_let_one_step_from_basic_type'; basic_typing_solver5. *) *)
+(*     (* eapply let_store_tyable; eauto. *) *)
+(*   - invclear H0; denotation_simp. *)
+(*     + do 3 (split; auto). intros. invclear H0. *)
+(*       { apply ctxrR_cons_over; denotation_simp; auto. admit. admit. *)
+(*         intros. *)
+(*         assert (({<[a:=c_x]> st}⟦{v:b|0|d|ϕ}⟧{Γ}) ({a := c_x}v u)) by auto. *)
+(*         assert ({<[a:=c_x]> st}⟦τ⟧{ Γ ++ [(z, {v:b|0|d|ϕ})] } ({a := c_x}t e)) by auto. *)
+(*         rewrite IHΓ in H3; mydestr; auto. *)
+(*         apply H8 in H1. admit. *)
+(*       } *)
+(*       { admit. } *)
+(*     + admit. *)
+(*   - destruct (classic (not_overbasety r)). *)
+(*     + constructor; try refinement_solver3. admit. *)
+(*     + auto_ty_exfalso. apply ctxrR_cons_over; try refinement_solver3. *)
+(*       intros. rewrite IHΓ. split. admit. split. admit. split. admit. *)
+(*       intros. admit. *)
+(* Admitted. *)
+
+Lemma rRctx_backward_under_forward: forall Γ st z τ_z (e: tm) τ,
+    not_overbasety τ ->
+    ~ not_overbasety τ_z ->
+    {st}⟦ τ ⟧{ Γ ++ [(z, τ_z)] } e ->
+      (∃ (u_hat: tm), {st}⟦ τ_z ⟧{ Γ } u_hat /\
+                        (forall (u: tm), {st}⟦ τ_z ⟧{ Γ } u ->
+                                    (∀ (v_u: value), u_hat ↪* v_u -> {st}⟦ { z:= v_u }r τ ⟧{ Γ } (tlete u (e ^t^ z)))
+                        )).
+Admitted.
+
+(* Lemma random_inhabitant_in_any_under: ∀ (τ: rty) (bst : bstate) n st, *)
+(*     not_overbasety τ -> *)
+(*     closed_rty n (dom _ st) τ -> *)
+(*     ({n;bst;st}⟦τ⟧) (random_inhabitant τ). *)
+(* Proof. *)
+(*   induction τ; intros; invclear H; mydestr. *)
+(*   - destruct B. *)
+(*     + split; simpl; auto. admit. split; auto. intros. admit. *)
+(*     + split; simpl; auto. apply mk_bool_gen_typable; auto. split; auto. intros. destruct c; invclear H. *)
+(*       apply mk_bool_gen_reduce_to_all_bool. *)
+(*   - denotation_simp. constructor; auto. admit. constructor; auto. *)
+(*     intros. *)
+(*     apply (termR_perserve_rR _ (random_inhabitant τ)); auto; try refinement_solver1. admit. *)
+(*     apply IHτ; refinement_solver1. *)
+(*   - denotation_simp. constructor; auto. admit. constructor; auto. *)
+(*     intros. *)
+(*     assert (exists (v_x: value), e_x ↪* v_x). admit. destruct H1. *)
+(*     apply (termR_perserve_rR _ (random_inhabitant τ2)); auto; try refinement_solver1. admit. *)
+(*     apply IHτ2; refinement_solver1. *)
+(* Admitted. *)
+
+(* Lemma denotation_weaken_empty: forall Γ (e: tm) τ (st: state), *)
+(*     not_overbasety τ -> *)
+(*     valid_rty τ -> *)
+(*     ok_dctx (dom _ st) Γ -> { st }⟦ τ ⟧ e -> {st}⟦ τ ⟧{ Γ } e. *)
+(* Proof. *)
+(*   induction Γ; intros; denotation_simp; mydestr. *)
+(*   constructor; auto. *)
+(*   destruct (classic (not_overbasety r)). *)
+(*   - constructor; auto; try refinement_solver1. *)
+(*     exists (random_inhabitant r); invclear H1; *)
+(*     assert (({0;b∅;st}⟦r⟧) (random_inhabitant r)) by *)
+(*       (intros; apply random_inhabitant_in_any_under; auto); *)
+(*     split; try (apply random_inhabitant_in_any_under; auto); intros. *)
+(*     + assert ([] ⊢t v_x ⋮v ⌊r⌋) as Hv_x by refinement_solver1. *)
+(*       destruct v_x; mydestr; simpl; try auto_ty_exfalso. *)
+(*       apply (termR_perserve_ctxrR _ _ e); auto. admit. *)
+(*       apply IHΓ; auto. denotation_simp. intros. rewrite rR_shadow_update_st; auto; refinement_solver1. *)
+(*       apply rR_regular1 in H2; mydestr. refinement_solver1. *)
+(*     + apply (termR_perserve_ctxrR _ _ e); auto. admit. *)
+(*       apply IHΓ; auto. denotation_simp. admit. admit. *)
+(*   - refinement_solver1. constructor; auto; try refinement_solver1. *)
+(*     intros. apply (termR_perserve_ctxrR _ _ e); auto. admit. *)
+(*     invclear H1; apply IHΓ; auto; try auto_ty_exfalso; try ok_dctx_solver_slow. *)
+(*     intros. rewrite rR_shadow_update_st; auto; refinement_solver1. *)
+(*     apply rR_regular1 in H2; mydestr. refinement_solver1. *)
+(* Admitted. *)
+
+(* Lemma denotation_weaken: forall Γ1 Γ3 (e: tm) τ (st: state) Γ2, *)
+(*     ctxrR_wf (dom _ st) (Γ1 ++ Γ2 ++ Γ3) τ -> {st}⟦ τ ⟧{ Γ1 ++ Γ3 } e -> {st}⟦ τ ⟧{ Γ1 ++ Γ2 ++ Γ3 } e. *)
+(* Proof. *)
+(*   intros. generalize dependent Γ2. *)
+(*   induction H0; intros; listctx_set_simpl. *)
+(*   - specialize (H b∅). invclear H; mydestr. denotation_simp. *)
+(*   induction Γ1; intros; listctx_set_simpl. *)
+(*   - admit. *)
+(*   -  *)
+
+(* Lemma err_exists_denotation_excluded: forall Γ b n (d: aset) (ϕ: refinement), *)
+(*     closed_rty 0 (dom aset (∅: state)) [v:b|n|d|ϕ] -> *)
+(*     ~ (⟦ [v: b | n | d | ϕ ] ⟧{ Γ } terr) -> (∃ (v: value), ⟦ {v: b | n | d | ϕ } ⟧{ Γ } v). *)
+(* Proof. *)
+(*   induction Γ; intros. *)
+(*   - destruct (classic (∃ v : value, (⟦{v:b|n|d|ϕ}⟧{ [] }) v)); auto; exfalso; apply H0; clear H0. *)
+(*     rewrite forall_iff_not_exists1 in H1. *)
+(*     constructor. intros. *)
+(*     do 2 constructor; auto. rewrite terr_reduction_iff_false_phi. *)
+(*     intros. intros Hf. *)
+(*     specialize (H1 c). apply H1. *)
+(*     constructor; auto. intros. constructor; auto. constructor; auto. *)
+(*     rewrite closed_rty_under_iff_over; auto. *)
+(*     exists c. constructor; auto. constructor; auto. *)
+(*     rewrite bound_in_refinement_0. apply Hf. refinement_solver1. *)
+(*   - mydestr. refinement_simp1. *)
+(*     destruct (classic (∃ v : value, (⟦{v:b|n|d|ϕ}⟧{ a :: Γ }) v)); auto; exfalso; apply H0; clear H0. *)
+(*     rewrite forall_iff_not_exists1 in H1. *)
+(*     mydestr. *)
+(*     constructor. *)
+
+
+(*     repeat match goal with *)
+(*            | [H: closed_rty _ _ _ |- bound_in_refinement _ _ ] => destruct H; mydestr *)
+(*            | [H: valid_rty _ |- bound_in_refinement _ _ ] => invclear H *)
+(*            | [H: wf_r _ _ ?ϕ |- bound_in_refinement _ ?ϕ ] =>  destruct H *)
+(*            end. *)
+(*     refinement_simp1; auto. *)
+(*     repeat match goal with *)
+(*     | [H: lc_rty_idx 0 [v:_|?n|_|_] |- _ ] => *)
+(*         match n with *)
+(*         | 0 => fail 1 *)
+(*         | _ =>  assert (n = 0) by (apply lc_rty_idx_under_0_is_0 in H; auto); subst *)
+(*         end *)
+(*     end. *)
+(*     repeat match goal with *)
+(*            | [H: closed_rty _ _ _ |- bound_in_refinement _ _ ] => destruct H; mydestr *)
+(*            | [H: valid_rty _ |- bound_in_refinement _ _ ] => invclear H *)
+(*            | [H: wf_r _ _ ?ϕ |- bound_in_refinement _ ?ϕ ] =>  destruct H *)
+(*            end. *)
+(*     assert (n = 0) by (apply lc_rty_idx_under_0_is_0 in H2; auto); subst. *)
+(*     invclear H2. *)
+(*     destruct H5.  *)
+(*     invclear H. *)
+(*  mydestr. invclear H. invclear H6. unfold bound_in_refinement in H5. *)
+(*     assert (closed_rty 0 ∅ [v:b|n|d|ϕ]). setoid_rewrite <- H2; auto. *)
+
+(*     setoid_rewrite H2 in H. *)
+
+(*     admit. auto. *)
+(*     intros. apply multistep_R. *)
+
+(*     constructor. *)
+(*     exfalso. apply H. constructor; intros. rewrite terr_inhabitant_iff_false_phi. *)
+
+
+(*   intros. destruct (classic (∃ v : value, (⟦[v:b|n|d|ϕ]⟧{Γ}) v)); auto. *)
+(*   exfalso. apply H. rewrite terr_inhabitant_iff_false_phi. *)
+
+(*   intro Hf. mydestr. invclear Hf. *)
+(*     + invclear H. denotation_simp. *)
+(*       match goal with *)
+(*       | [H: ∀ c, [] ⊢t (vconst c) ⋮v _ → _ _ ∅ c → terr ↪* (tvalue (vconst c)) |- _ ] => idtac H *)
+(*       end. *)
+(*       rewrite terr_inhabitant_implies_false_phi in H4. *)
+(*       apply H4 in H7. *)
+(*       repeat match goal with *)
+(*       | [H: _ ⊢t ?v ⋮v (TBase _) |- _ ] => *)
+(*           match v with *)
+(*           | vconst _ => fail 1 *)
+(*           | _ => set H7 as Htmp; apply empty_basic_typing_base_const_exists in Htmp; mydestr; subst *)
+(*           end *)
+(*       end. *)
+(*       set H7 as Htmp; apply empty_basic_typing_base_const_exists in Htmp; mydestr; subst. *)
+(*       match goal with *)
+(*       | [H: _ ⊢t (tvalue ?v) ⋮t _ |- _ ] => invclear H *)
+(*       end. *)
+
+(*       apply empty_basic_typing_base_const_exists in H. *)
+
+(*        specialize (H1 b∅). *)
+(*       invclear H0. invclear H1. mydestr. *)
+(* Admitted. *)
